first stab at proofs

src/Bedrock/Compiler.v
@@ -3,6 +3,7 @@ Require Import Coq.Lists.List.
 Require bedrock2.Syntax.
 Require bedrock2.Semantics.
 Require bedrock2.BasicC64Semantics. (* for debugging *)
+Require bedrock2.WeakestPrecondition.
 Require Import Crypto.Util.ZRange.
 Require Import Crypto.BoundsPipeline.
 Require Import Crypto.Util.Notations.
@@ -18,6 +19,12 @@ Module Compiler.
             (ident_to_funname : forall t, ident.ident t -> Syntax.funname).
     Local Notation cexpr := (@Language.Compilers.expr.expr base.type ident.ident).
     Local Notation maxint := (2 ^ Semantics.width).
+
+    (* Notations for commonly-used types *)
+    Local Notation type_nat := (type.base (base.type.type_base base.type.nat)).
+    Local Notation type_Z := (type.base (base.type.type_base base.type.Z)).
+    Local Notation type_ZZ :=
+      (type.base (base.type.prod (base.type.type_base base.type.Z) (base.type.type_base base.type.Z))).
 
     (* cexpr typing cheat sheet:
          Language.Compilers.type === type.type := base (of base.type) or arrow (recursive type.type)
@@ -106,11 +113,6 @@ Module Compiler.
 
     Definition max_range : zrange := {| lower := 0; upper := 2 ^ Semantics.width |}.
     Definition range_good (r : zrange) : bool := is_tighter_than_bool r max_range.
-
-    Local Notation type_nat := (type.base (base.type.type_base base.type.nat)).
-    Local Notation type_Z := (type.base (base.type.type_base base.type.Z)).
-    Local Notation type_ZZ :=
-      (type.base (base.type.prod (base.type.type_base base.type.Z) (base.type.type_base base.type.Z))).
 
     (* checks that the expression is either a) a literal nat or Z that
     falls within the allowed range or b) an expression surrounded by
@@ -622,4 +624,158 @@ Module Compiler.
     Eval lazy in (fun c x y => of_expr (test_expr6 c x y) tt "ret").
     *)
   End debug.
+
+  Section Proofs.
+    Context {p : Semantics.parameters}
+            (next_varname : Syntax.varname -> Syntax.varname)
+            (error : Syntax.expr.expr)
+            (ident_to_funname : forall t, ident.ident t -> Syntax.funname).
+    Local Notation cexpr := (@Language.Compilers.expr.expr base.type ident.ident).
+    Local Notation cExpr := (@Language.Compilers.expr.Expr base.type ident.ident).
+    Local Notation maxint := (2 ^ Semantics.width).
+
+    (* Notations for commonly-used types *)
+    Local Notation type_nat := (type.base (base.type.type_base base.type.nat)).
+    Local Notation type_Z := (type.base (base.type.type_base base.type.Z)).
+    Local Notation type_ZZ :=
+      (type.base (base.type.prod (base.type.type_base base.type.Z) (base.type.type_base base.type.Z))).
+
+    (* TODO : fill these in *)
+    Axiom valid_carry_expr : forall {t}, @cexpr var t -> Prop.
+    Axiom valid_inner_expr : forall {t}, @cexpr var t -> Prop.
+
+    (* states whether the expression is acceptable input for [of_expr] *)
+    Inductive valid_expr : forall {t}, @cexpr var t -> Prop :=
+    | valid_carry_let :
+        forall t x f,
+          valid_carry_expr x ->
+          (forall names, valid_expr (f names)) ->
+          valid_expr (expr.LetIn (A:=type_ZZ) (B:=t) x f)
+    | valid_let :
+        forall t1 t2 x f,
+          valid_inner_expr x ->
+          (forall names, valid_expr (f names)) ->
+          valid_expr (expr.LetIn (A:=type.base t1) (B:=t2) x f)
+    | valid_cons :
+        forall x l,
+          valid_inner_expr x ->
+          valid_expr l ->
+          valid_expr (expr.App (expr.App (expr.Ident (@ident.cons base.type.Z)) x) l)
+    | valid_nil :
+        valid_expr (expr.Ident (@ident.nil base.type.Z))
+    | valid_app :
+        forall s d f x,
+          valid_inner_expr (expr.App (s:=type.base s) (d:=type.base d) f x) ->
+          valid_expr (expr.App f x)
+    | valid_ident :
+        forall t i,
+          valid_inner_expr (expr.Ident (t:=type.base t) i) ->
+          valid_expr (expr.Ident i)
+    | valid_var :
+        forall t x,
+          valid_inner_expr (expr.Var (t:=type.base t) x) ->
+          valid_expr (expr.Var x)
+    | valid_abs :
+        forall s d f,
+          (forall names, valid_expr (f names)) ->
+          valid_expr (expr.Abs (s:=type.base s) (d:=d) f)
+    .
+
+    (* convert expressions that are expected to be all variable names from var
+       to the flat list format expected by bedrock for function input/output *)
+    Fixpoint base_var_to_list {t} : base_var t -> option (list Syntax.varname) :=
+      match t with
+      | base.type.prod a b =>
+        fun x : base_var a * base_var b =>
+          Option.bind (base_var_to_list (fst x))
+                      (fun lx => option_map (app lx) (base_var_to_list (snd x)))
+      | base.type.list (base.type.type_base base.type.Z) =>
+        fun x : Syntax.expr.expr =>
+          match x with
+          | Syntax.expr.var n => Some [n]
+          | _ => None (* fail if list location is any expr other than a variable *)
+          end
+      | _ => fun x : Syntax.varname => Some [x]
+      end.
+    Fixpoint var_to_list {t} : var t -> option (list Syntax.varname) :=
+      match t with
+      | type.base a => fun x => base_var_to_list x
+      | type.arrow a b => fun _ => None (* can't convert a function to a varname *)
+      end.
+
+    (* convert the type of arguments from the nested for_each_lhs_of_arrow
+       construction to a flat list
+
+       of_expr expects type.for_each_lhs_of_arrow, which gives you a var for
+       each argument, which for the most part gives you Syntax.expr.expr (and
+       functions from var -> var if the argument is a function)
+
+       bedrock wants to get a list of variable names, which is a more
+       restrictive requirement; instead of expr.expr, we would want everything
+       to be a Syntax.expr.var. This function returns [None] if the more
+       restrictive condition is not met. *)
+    Fixpoint args_to_list {t}
+      : type.for_each_lhs_of_arrow var t -> option (list Syntax.varname) :=
+      match t with
+      | type.base _ => fun _ : unit => Some nil
+      | type.arrow (type.base s) d =>
+        fun args : base_var s * type.for_each_lhs_of_arrow var d =>
+          Option.bind
+            (base_var_to_list (fst args))
+            (fun x =>
+               option_map
+                 (app x)
+                 (args_to_list (snd args)))
+      | type.arrow (type.arrow s d1) d2 => fun _ => None (* can't have function arguments *)
+      end.
+
+    (* bedrock postcondition stating that the bedrock result is equivalent to
+       the fiat-crypto result *)
+    Inductive results_equivalent :
+      forall t, type.interp base.interp t ->
+                @Interface.map.rep _ _ Semantics.mem ->
+                  list Interface.word.rep -> Prop :=
+    | equiv_prod :
+        forall a b res mem rets1 rets2,
+          results_equivalent (type.base a) (fst res) mem rets1 ->
+          results_equivalent (type.base b) (snd res) mem rets2 ->
+          results_equivalent (type.base (base.type.prod a b)) res mem (rets1 ++ rets2)
+    | equiv_list :
+        forall (res : list Z) mem ret,
+          (* for all 0 <= i < list length, the value in memory at ret+i matches the list *)
+          Forall (fun i =>
+                    let addr := Interface.word.add ret (Interface.word.of_Z (Z.of_nat i)) in
+                    exists w,
+                      Interface.map.get mem addr = Some w /\
+                      Interface.word.unsigned w = nth_default 0 res i)
+                 (seq 0 (length res)) ->
+          results_equivalent (type.base (base.type.list base.type.Z)) res mem [ret]
+    | equiv_Z :
+        forall (res : Z) mem w,
+          Interface.word.unsigned w = res ->
+          results_equivalent type_Z res mem [w]
+    .
+
+    (* cast-outside-of-range with behavior similar to words *)
+    Definition cast_oor_truncate (r : zrange) (x : Z) : Z :=
+      (Z.max (lower r) x) mod (upper r + 1).
+
+    Lemma of_expr_correct {t} (e : @cExpr t) :
+      valid_expr (e var) ->
+      forall nextname argnames rets,
+      forall funnames fname innames outnames trace mem args,
+        var_to_list rets = Some outnames ->
+        args_to_list argnames = Some innames ->
+        let of_expre : Syntax.cmd.cmd :=
+            snd (of_expr next_varname error (e var) nextname argnames rets) in
+        let interpe : type.interp base.interp t :=
+            expr.interp (interp_base_type:=base.interp)
+                        (@ident.gen_interp cast_oor_truncate) (e _) in
+        In (fname, (innames, outnames, of_expre)) funnames ->
+        WeakestPrecondition.call
+          funnames fname trace mem args (fun _ => results_equivalent _ interpe).
+    Proof.
+      (* TODO : look at Jason's final correctness theorem, make sure this short-circuits correctly. *)
+    Admitted.
+  End Proofs.
 End Compiler.
